LeanYjs/ActorId.lean
@@ -1,0 +1,12 @@
+def ActorId := Nat
+
+instance : LT ActorId where
+  lt x y := Nat.lt x y
+
+instance : DecidableRel (· < · : ActorId → ActorId → Prop) := by
+  intros x y
+  unfold ActorId at x y
+  apply (inferInstance : Decidable (x < y))
+
+instance ActorIdOfNat n : OfNat ActorId n where
+  ofNat := n
