LeanYjs/ItemPartialOrder.lean
@@ -1,0 +1,48 @@
+import LeanYjs.ActorId
+import LeanYjs.YItem
+import Mathlib.Order.Defs.Unbundled
+
+open Relation
+
+variable (A : Type) [BEq A]
+
+inductive YjsPtrLt : YjsPtr A -> YjsPtr A -> Prop where
+  | lt_left : forall o r id c, YjsPtrLt o (YjsItem.item o r id c)
+  | lt_right : forall o r id c, YjsPtrLt (YjsItem.item o r id c) r
+  | lt_first : forall item, YjsPtrLt YjsPtr.first (YjsPtr.itemPtr item)
+  | lt_last : forall item, YjsPtrLt (YjsPtr.itemPtr item) YjsPtr.last
+
+def YjsPtrLtTrans := TransGen (r := YjsPtrLt A)
+
+inductive YjsReanchableOne : YjsPtr A -> YjsPtr A -> Prop where
+  | reachable : forall o r id c, YjsReanchableOne (YjsItem.item o r id c) o
+  | reachable_right : forall o r id c, YjsReanchableOne (YjsItem.item o r id c) r
+
+def YjsReanchable := TransGen (r := YjsReanchableOne A)
+
+inductive YjsPtrLt2 : YjsPtr A -> YjsPtr A -> Prop where
+  | lt_trans x y : YjsPtrLtTrans A x y -> YjsPtrLt2 x y
+  /-
+    if t is reachable, then t isn't between o and r
+    This means that (YjsItem.item o r id c) is neightbor of l and r at least when inserted.
+  -/
+  | lt_reachable1 o r id c t :
+    YjsReanchable A (YjsItem.item o r id c) t ->
+    YjsPtrLt2 t r ->
+    YjsPtrLt2 t o
+  | lt_reachable2 o r id c t :
+    YjsReanchable A (YjsItem.item o r id c) t ->
+    YjsPtrLt2 o t ->
+    YjsPtrLt2 r t
+
+variable (P : YjsItem A -> Prop)
+
+def YjsItemSubset := { i : YjsItem A // P i }
+
+def YjsItemSubsetLeq (x y : YjsItemSubset _ P) : Prop :=
+  x = y ∨ YjsPtrLtTrans A (↑x.1) (↑y.1)
+
+def ValidYjsSubsetPred (P : YjsItem A -> Prop) :=
+  (∀ (o : YjsItem A) r id c, P (YjsItem.item o r id c) -> P o) ∧
+  (∀ o (r : YjsItem A) id c, P (YjsItem.item o r id c) -> P r) ∧
+  IsPartialOrder (YjsItemSubset _ P ) (YjsItemSubsetLeq _ _)
