LeanYjs/YItem.lean
@@ -1,0 +1,65 @@
+import LeanYjs.ActorId
+
+variable (A : Type) [BEq A]
+
+mutual
+inductive YjsPtr : Type where
+  | itemPtr : YjsItem -> YjsPtr
+  | first : YjsPtr
+  | last : YjsPtr
+
+inductive YjsItem : Type where
+| item (origin : YjsPtr) (rightOrigin : YjsPtr) : ActorId -> A -> YjsItem
+end
+
+def YjsItem.origin {A : Type} (item : YjsItem A) : YjsPtr A :=
+  match item with
+  | YjsItem.item origin _ _ _ => origin
+
+def YjsItem.rightOrigin {A : Type} (item : YjsItem A) : YjsPtr A :=
+  match item with
+  | YjsItem.item _ rightOrigin _ _ => rightOrigin
+
+mutual
+def YjsPtr.size {A : Type} (x : YjsPtr A) :=
+  match x with
+  | YjsPtr.itemPtr item => item.size + 1
+  | YjsPtr.first => 0
+  | YjsPtr.last => 0
+
+def YjsItem.size {A : Type} (item : YjsItem A) :=
+  match item with
+  | YjsItem.item origin rightOrigin _ _ =>
+    origin.size + rightOrigin.size + 2
+end
+
+instance : BEq ActorId where
+  beq x y := by
+    unfold ActorId at x y
+    apply Nat.beq x y
+
+mutual
+def yjsItemEq (x y : YjsItem A) : Bool :=
+  match x, y with
+  | YjsItem.item origin1 rightOrigin1 id1 c1, YjsItem.item origin2 rightOrigin2 id2 c2 =>
+    yjsPtrEq origin1 origin2 && yjsPtrEq rightOrigin1 rightOrigin2 && id1 == id2 && c1 == c2
+
+def yjsPtrEq (x y : YjsPtr A) : Bool :=
+  match x, y with
+  | YjsPtr.itemPtr item1, YjsPtr.itemPtr item2 => yjsItemEq item1 item2
+  | YjsPtr.first, YjsPtr.first => true
+  | YjsPtr.last, YjsPtr.last => true
+  | _, _ => false
+end
+
+instance BEqYjsItem : BEq (YjsItem A) where
+  beq := yjsItemEq _
+
+instance BEqYjsPtr : BEq (@YjsPtr A) where
+  beq := yjsPtrEq _
+
+instance : Coe (YjsItem A) (YjsPtr A) where
+  coe item := YjsPtr.itemPtr item
+
+def YjsItem.id {A : Type} : YjsItem A -> ActorId
+| YjsItem.item _ _ id _ => id
